\newpage
\section{Basis Transformation Coefficient} \label{app:basistrafo}
arrows ($\uparrow\,,\, \downarrow$) correspond to spin (up, down), while $+$ and $-$ correspond to positive and negative helicity, respectively
\begin{align} \label{eq:basistrafo_bd}
    H_{RKKY} =  \sum_{\substack{i, k,k'\\ \lambda, \lambda'}} &\frac{J}{N} \frac{e^{i(k-k')r_i}}{2\sqrt{|\gamma(k)||\gamma(k')|}} \\ \nonumber
    \times \left[ \right. & \left. \delta_{\lambda,\lambda'} \left( S^i_z\sqrt{|\gamma_k|+\lambda\gamma_{k,z}}\sqrt{|\gamma_{k'}|+\lambda\gamma_{k',z}}- S^i_z\sqrt{|\gamma_k|-\lambda\gamma_{k,z}}\sqrt{|\gamma_{k'}|-\lambda\gamma_{k',z}} \right. \\ \nonumber
    \left. \right. &\left. + \frac{\gamma_{k',x} + i \gamma_{k',y}}{\sqrt{\gamma^2_{k',x} + \gamma^2_{k',y}}} (S^i_x-iS_y^i)\lambda \sqrt{|\gamma_{k}|+\lambda\gamma_{k,z}}\sqrt{|\gamma_{k'}|-\lambda\gamma_{k',z}}\right. \\ \nonumber
    \left. \right. &\left.
    + \frac{\gamma_{k,x} - i \gamma_{k,y}}{\sqrt{\gamma^2_{k,x} + \gamma^2_{k,y}}} (S^i_x+iS_y^i)\lambda \sqrt{|\gamma_{k}|-\lambda\gamma_{k,z}}\sqrt{|\gamma_{k'}|+\lambda\gamma_{k',z}}
    \right) \right. \\ \nonumber
    \left.  +\right. & \left. \delta_{-\lambda, \lambda'}\left( S^i_z\sqrt{|\gamma_k|+\lambda\gamma_{k,z}}\sqrt{|\gamma_{k'}|-\lambda\gamma_{k',z}} + S^i_z\sqrt{|\gamma_k|-\lambda\gamma_{k,z}}\sqrt{|\gamma_{k'}|+\lambda\gamma_{k',z}} \right. \\ \nonumber
    \left. \right. & \left.
    - \frac{\gamma_{k',x} + i \gamma_{k',y}}{\sqrt{\gamma^2_{k',x} + \gamma^2_{k',y}}} (S^i_x-iS_y^i)\lambda \sqrt{|\gamma_{k}|+\lambda\gamma_{k,z}}\sqrt{|\gamma_{k'}|+\lambda\gamma_{k',z}}\right. \\ \nonumber
    \left. \right. &\left.
    + \frac{\gamma_{k,x} - i \gamma_{k,y}}{\sqrt{\gamma^2_{k,x} + \gamma^2_{k,y}}} (S^i_x+iS_y^i)\lambda \sqrt{|\gamma_{k}|-\lambda\gamma_{k,z}}\sqrt{|\gamma_{k'}|-\lambda\gamma_{k',z}} \right) \right] b^{\dag}_{k,\lambda}b_{k',\lambda'}
\end{align}

for Rashba-type SOC the expression simplifies to

\begin{align} \nonumber
    H_{RKKY} =  \sum_{\substack{i, k,k'\\ \lambda, \lambda'}} &\frac{J}{N} \frac{e^{i(k-k')r_i}}{2 \lambda}
    \times \left[  \delta_{\lambda,\lambda'} \left(  \frac{\gamma_{k',x} + i \gamma_{k',y}}{\sqrt{\gamma^2_{k',x} + \gamma^2_{k',y}}} (S^i_x-iS_y^i)   + \frac{\gamma_{k,x} - i \gamma_{k,y}}{\sqrt{\gamma^2_{k,x} + \gamma^2_{k,y}}} (S^i_x+iS_y^i)
    \right) \right. \\ \nonumber
    \left.  +\right. & \left. \delta_{-\lambda, \lambda'}\left( 2  \lambda S^i_z
    - \frac{\gamma_{k',x} + i \gamma_{k',y}}{\sqrt{\gamma^2_{k',x} + \gamma^2_{k',y}}} (S^i_x-iS_y^i)
    + \frac{\gamma_{k,x} - i \gamma_{k,y}}{\sqrt{\gamma^2_{k,x} + \gamma^2_{k,y}}} (S^i_x+iS_y^i) \right) \right] b^{\dag}_{k,\lambda}b_{k',\lambda'}
\end{align}
