\newpage
\section{Commutators}
\subsection{$[S,H_0]$} \label{app:commutator1}
With using the anti-commutation relations of the $d^{[\dag]}$-operators, this commutator reads:
\begin{align}\nonumber
    \sum_{\substack{k,k'\\ \lambda, \lambda' }} \sum_{q,\beta} &\left[  A_{\substack{i,k,k'\\ \lambda, \lambda'}}^{ \gamma} d^{\dag}_{k,\lambda} d_{k', \lambda'}+ B_{\substack{i,k,k'\\ \lambda, \lambda'}}^{ \gamma} d_{-k,\lambda} d^{\dag}_{-k', \lambda'} \right. \\
    & \left. + C_{\substack{i,k,k'\\ \lambda, \lambda'}}^{ \gamma} d_{-k,\lambda} d_{k', \lambda'}+ D_{\substack{i,k,k'\\ \lambda, \lambda'}}^{ \gamma} d^{\dag}_{k,\lambda} d^{\dag}_{-k', \lambda'}\, , \, E_{q,\beta} d^{\dag}_{q,\beta} d_{q,\beta} \right] \\ \nonumber
    =  - \sum_{\substack{k,k'\\ \lambda, \lambda' }} \sum_{q,\beta} 
    &\left( A_{\substack{i,k,k'\\ \lambda, \lambda'}}^{ \gamma}\,E_{q,\beta} \left( d^{\dag}_{q,\beta} d_{k', \lambda'} \{ d_{q,\beta}\, , \, d^{\dag}_{k, \lambda} \}- d^{\dag}_{k,\lambda} d_{q, \beta} \{ d^{\dag}_{q,\beta}\, , \, d_{k', \lambda'} \}  \right) \right. \\ \nonumber
    &\left. + B_{\substack{i,k,k'\\ \lambda, \lambda'}}^{ \gamma}\,E_{q,\beta} \left( -d^{\dag}_{q,\beta} d_{-k, \lambda} \{ d_{q,\beta}\, , \, d^{\dag}_{-k', \lambda'} \} + d^{\dag}_{-k',\lambda'} d_{q, \beta} \{ d^{\dag}_{q,\beta}\, , \, d_{-k, \lambda} \}  \right) \right.\\ \nonumber
    &\left. + C_{\substack{i,k,k'\\ \lambda, \lambda'}}^{ \gamma}\,E_{q,\beta} \left( d_{k',\lambda'} d_{q, \beta} \{ d^{\dag}_{q,\beta}\, , \, d_{-k, \lambda} \} - d_{-k,\lambda} d_{q, \beta} \{ d^{\dag}_{q,\beta}\, , \, d_{k', \lambda'} \}  \right)\right.\\ \nonumber
    &\left. + D_{\substack{i,k,k'\\ \lambda, \lambda'}}^{ \gamma}\,E_{q,\beta} \left( d^{\dag}_{q,\beta} d^{\dag}_{-k', \lambda'} \{ d_{q,\beta}\, , \, d^{\dag}_{k, \lambda} \} - d^{\dag}_{q,\beta} d^{\dag}_{k, \lambda} \{ d_{q,\beta}\, , \, d^{\dag}_{-k', \lambda'} \}  \right) \right) \\ \nonumber
    = - \sum_{\substack{k,k'\\ \lambda, \lambda' }} 
    & \left( A_{\substack{i,k,k'\\ \lambda, \lambda'}}^{ \gamma} d^{\dag}_{k,\lambda} d_{k', \lambda'} (E_{k,\lambda} - E_{k'\lambda'}) 
    + B_{\substack{i,k,k'\\ \lambda, \lambda'}}^{ \gamma} d_{-k,\lambda} d^{\dag}_{-k', \lambda'} ( E_{-k',\lambda'} - E_{-k,\lambda} ) \right. \\
    &\left. - C_{\substack{i,k,k'\\ \lambda, \lambda'}}^{ \gamma} d_{-k,\lambda} d_{k', \lambda'}(E_{-k, \lambda} + E_{k'\lambda'})
    + D_{\substack{i,k,k'\\ \lambda, \lambda'}}^{ \gamma} d^{\dag}_{k,\lambda} d^{\dag}_{-k', \lambda'} (E_{k,\lambda} + E_{-k', \lambda'}) \right)
\end{align}

\subsection{$[S,H_{RKKY}]$} \label{app:commutator2}
With disregarding all terms that contain either $d_{k,\lambda} d_{k', \lambda'}$ or $d^{\dag}_{k,\lambda} d^{\dag}_{k', \lambda'}$, sinee they are not going to contribute to the expectation value and are therefore of no interest in this case, this commutator reads:

\begin{align}\nonumber
    [ \sum_{\substack{q,q'\\ \beta, \beta' }} A_{\substack{j,q,q'\\ \beta, \beta'}}^{ \gamma} d^{\dag}_{q,\beta} d_{q', \beta'}
    &+ B_{\substack{j,q,q'\\ \beta, \beta'}}^{ \gamma} d_{-q,\beta} d^{\dag}_{-q', \beta'}
    + C_{\substack{j,q,q'\\ \beta, \beta'}}^{ \gamma} d_{-q,\beta} d_{q', \beta'}
    + D_{\substack{j,q,q'\\ \beta, \beta'}}^{ \gamma} d^{\dag}_{q,\beta} d^{\dag}_{-q', \beta'} \, , \\ \nonumber
    \sum_{\substack{i, k,k'\\ \lambda, \lambda' }} T^{ \gamma}_{i,k, k', \lambda, \lambda'} &\left(
    \eta^{\dag}_{k, \lambda}\eta_{k',\lambda'} d^{\dag}_{k,\lambda}d_{k',\lambda'}
    + \nu_{k,\lambda} \nu^{\dag}_{k',\lambda'} d^{\dag}_{k,\lambda}d_{-k',\lambda'}
    + \nu_{k,\lambda}\eta_{k',\lambda'} d^{\dag}_{-k,\lambda}d_{k',\lambda'} 
    + \eta^{\dag}_{k,\lambda} \nu^{\dag}_{k',\lambda'} d^{\dag}_{k,\lambda}d_{-k',\lambda'} \right) ]\\ \nonumber
    = \sum_{\substack{q,q', k, k' \\ \beta, \beta', \lambda, \lambda' }} - A_{\substack{j,q,q'\\ \beta, \beta'}}^{ \gamma} &\left(T^{ \gamma}_{i,k, q, \lambda, \beta}\eta^{\dag}_{k, \lambda}\eta_{q,\beta} d^{\dag}_{k,\lambda}d_{q',\beta'} 
    - T^{ \gamma}_{i,q', k', \beta', \lambda'}\eta^{\dag}_{q', \beta'}\eta_{k',\lambda'} d^{\dag}_{q,\beta}d_{k',\lambda'} \right. \\ \nonumber
    &\left. - T^{ \gamma}_{i,k, -q', \lambda, \beta'}\nu_{k,\lambda} \nu^{\dag}_{-q',\beta'} d_{-k,\lambda}d^{\dag}_{q,\beta} 
    + T^{ \gamma}_{i,-q, k', \beta, \lambda'}\nu_{-q,\beta} \nu^{\dag}_{k,\lambda} d_{q',\beta'}d^{\dag}_{-k',\lambda'} \right) \\ \nonumber
    - B_{\substack{j,q,q'\\ \beta, \beta'}}^{ \gamma}&\left(-T^{ \gamma}_{i,k, -q', \lambda, \beta'}\eta^{\dag}_{k, \lambda}\eta_{-q',\beta'} d^{\dag}_{k,\lambda}d_{-q,\beta} 
    + T^{ \gamma}_{i,-q, k', \beta, \lambda'}\eta^{\dag}_{-q, \beta}\eta_{k',\lambda'} d^{\dag}_{-q',\beta'}d_{k',\lambda'} \right. \\ \nonumber
    &\left. + T^{ \gamma}_{i,k, q, \lambda, \beta}\nu_{k,\lambda} \nu^{\dag}_{q,\beta} d_{-k,\lambda}d^{\dag}_{-q',\beta'} 
    - T^{ \gamma}_{i,q', k', \beta', \lambda'}\nu_{q',\beta'} \nu^{\dag}_{k',\lambda'} d_{-q,\beta}d^{\dag}_{-k',\lambda'} \right) \\ \nonumber
    - C_{\substack{j,q,q'\\ \beta, \beta'}}^{ \gamma}&\left(T^{ \gamma}_{i,k, q, \lambda, \beta}\eta^{\dag}_{k, \lambda}\nu^{\dag}_{q,\beta} d^{\dag}_{k,\lambda}d_{q',\beta'} 
    - T^{ \gamma}_{i,k, -q', \lambda, \beta'}\eta^{\dag}_{k, \lambda}\nu^{\dag}_{-q',\beta'} d^{\dag}_{k, \lambda}d_{-q, \beta} \right. \\ \nonumber
    &\left. + T^{ \gamma}_{i,-q, k', \beta, \lambda'}\eta^{\dag}_{-q,\beta} \nu^{\dag}_{k', \lambda'} d_{q',\beta'}d^{\dag}_{-k',\lambda'} 
    - T^{ \gamma}_{i,q', k', \beta', \lambda'}\eta^{\dag}_{q',\beta'} \nu^{\dag}_{k',\lambda'} d_{-q,\beta}d^{\dag}_{-k',\lambda'} \right) \\ \nonumber
    - D_{\substack{j,q,q'\\ \beta, \beta'}}^{ \gamma}&\left(T^{ \gamma}_{i,k, q, \lambda, \beta}\nu_{k, \lambda}\eta_{q,\beta} d_{-k,\lambda} d^{\dag}_{-q',\beta'}
    - T^{ \gamma}_{i,k, -q', \lambda, \beta'}\nu_{k, \lambda}\eta_{-q',\beta'} d_{-k, \lambda}d^{\dag}_{q, \beta} \right. \\ \nonumber
    &\left. + T^{ \gamma}_{i,-q, k', \beta, \lambda'}\nu_{-q,\beta} \eta_{k', \lambda'} d^{\dag}_{-q',\beta'} d_{k',\lambda'}
    - T^{ \gamma}_{i,q', k', \beta', \lambda'}\nu_{q',\beta'} \eta_{k',\lambda'} d^{\dag}_{q, \beta}d_{k', \lambda'} \right) \\ \nonumber
\end{align}